Commenting and cleaning ProbabilismWP (done)

ProbabilismWP.fst
@@ -54,7 +54,7 @@ let prob_wp_eqI #a (wp1 wp2: prob_wp a) :
 // (I.e., they satisfy "forall post, sum_{x:a} f(x)post(x) >= w(post).)
 // TODO: A refinement has to be added with that condition
 let prob a (w:prob_wp a): Tot Type0 =
-  distribution a // TODO: require w to hold
+  distribution a
 
 // Wp corresponding to "prob_return x"
 let prob_wreturn #a x : prob_wp a = (fun post -> post x)
@@ -67,10 +67,6 @@ let prob_return a (x:a) : prob a (prob_wreturn x) =
 let prob_wbind #a #b (w1:prob_wp a) (w2:a -> prob_wp b) : prob_wp b = 
   fun post -> w1 (fun x -> w2 x post)
 
-// TODO: document or remove
-let prob_wbind_beta #a #b (w1:prob_wp a) (w2:a -> prob_wp b) (post:prob_post b) :
-  Lemma (prob_wbind w1 w2 post == w1 (fun x -> w2 x post)) = ()
-
 // Semantics of "let x = p1 in p2 x"
 let prob_bind a b (w1:prob_wp a) (w2:a -> prob_wp b)
       (f: prob a w1) (g: (x:a -> prob b (w2 x))) : prob b (prob_wbind w1 w2) =
@@ -78,17 +74,6 @@ let prob_bind a b (w1:prob_wp a) (w2:a -> prob_wp b)
 
 // w1 is a more restrictive wp than w2
 let stronger #a (w1 w2:prob_wp a) = forall post. w1 post >=. w2 post
-
-// TODO: document or remove
-let strongerI #a (w1 w2:prob_wp a) :
-  Lemma (requires forall post. w1 post >=. w2 post)
-        (ensures w1 `stronger` w2) = ()
-
-// TODO: document or remove
-let prob_wp_stronger_eq #a (w1 w2:prob_wp a) :
-    Lemma (requires w1 `stronger` w2 /\ w2 `stronger` w1)
-    	  (ensures w1 == w2) = 
-    assert (w1 == w2) by (apply_lemma (`prob_wp_eqI))
 
 // Weakening in the PROB effect: takes "f:prob a w1" and returns the same f with a different type "prob a w2",
 // assuming w2 is a weaker wp than w2
@@ -115,13 +100,6 @@ layered_effect { PROB : (a:Type) -> (wp:prob_wp a) -> Effect with
   if_then_else = ite_prob
   }
 
-// TODO: document or remove
-assume val real_numbers_complete: unit -> Lemma(
-  forall (p: real->bool) low high.
-  p low ==> not (p high) ==> (forall x y. x >=. y ==> p x ==> p y) ==>
-  (exists sup. (forall x. x <. sup ==> p x) /\ (forall x. x >. sup ==> not (p x))))
-
-
 // "largest p" is the largest real satisfying p
 // TODO: Add ensures to state that it returns the largest real
 // TODO: Add requires to enforce conditions of p that are needed for that real to exist
@@ -142,8 +120,7 @@ let lift_pure_prob_wp #a (wp:pure_wp a) : prob_wp a =
 
 // Given pure program f, returns the corresponding probabilistic program "return f"
 let lift_pure_prob a (wp:pure_wp a) (f: eqtype_as_type unit -> PURE a wp) : 
-   prob a (lift_pure_prob_wp wp) =
-   assume False; // TODO
+   prob a (lift_pure_prob_wp wp) by (admit_all()) =
    point_distribution (f ())
 
 // Using lift_pure_prob, we tell F* how to transform a PURE effect
@@ -173,9 +150,6 @@ let test1 () : PROB bool (fun post -> (post true +. post false) /. two) = coin (
 // Testing if things work
 let test2 () : ProbAny bool = coin ()
 
-// XXXXXXXXXXXXXX
-
-
 // Attempt at telling SMT how to simplify a bind-return combination.
 // But the SMTPat gives a warning, so probably the match is too
 // higher-order for SMT
@@ -190,7 +164,7 @@ assume val return_bind (#a #b:Type) (x:a) (wp2:a -> prob_wp b) : Lemma(prob_wbin
   [SMTPat (prob_wbind (prob_wreturn x) wp2)]
 
 // Testing if things work.
-// Interestingly, if we inline f here, this does not immediately typecheck any more (see test8b).
+// Interestingly, if we inline f here, this does not immediately typecheck any more (see test8 which does not work yet, even with simplifier).
 let f (b:bool) : nat = if b then 0 else 1
 let test5 () : PROB nat (fun post -> (post 0 +. post 1) /. two) =
   let c : bool = coin() in f c
@@ -199,133 +173,102 @@ let test5 () : PROB nat (fun post -> (post 0 +. post 1) /. two) =
 let test6 () : PROB nat (fun p -> p 0) =
   let c : bool = coin() in 0
 
-//let bool_simp1 () : Lemma((true = true) == true) = ()
-//let bool_simp2 () : Lemma((false = true) == false) = ()
-//let bool_simp3 () : Lemma(~true == False) = ()
-//let bool_simp4 () : Lemma(~false == True) = ()
+// Like if, but the condition is Type0, not bool.
+// Useful for expressing rewriting rules (e.g., ifte_lift).
+// But it's equivalent to StrongExcludedMiddle, so maybe better try to get rid ofit
+let ifte (#a:Type) (c:Type0) (t:a) (e:a) : GTot a = 
+    if (FStar.StrongExcludedMiddle.strong_excluded_middle c) then t else e
 
 
-assume val ifte : #(a:Type) -> (c:Type0) -> (t:a) -> (e:a) -> a
+// The PURE wp corresponding to "admit()" 
+let pure_admit_wp (a:Type) : pure_wp a by (norm [delta]) = (fun (p: pure_post a) -> True)
 
-let largest_single c f : 
-Lemma(largest (fun (p:pr) -> c ==> f p) == ifte c (largest f) 1.0R)
-[SMTPat (largest (fun (p:pr) -> c ==> f p))]
-= assume False
+// The PROB wp corresponding to "admit()".
+// Some inconsistency here. For this to be meaningful, need to use extended reals instead of reals in preconditions.
+// I don't bother to fix this because probably I prefer the Hoare-approach anyway which does not have this problem.
+assume val prob_admit_wp : (a:Type) -> prob_wp a (* fun _ -> infinity *)
 
-(* let simp1 #a k f :
-Lemma((forall k. (forall (x:a). f x ==> k x) ==> (forall (x:a). k x))
-==
-(forall (x:a). f x))
-[SMTPat (forall k. (forall (x:a). f x ==> k x) ==> (forall (x:a). k x))]
-= assume False *)
-
-let probr #a (x:a) : PROB a (prob_wreturn x) by (admit_all()) = x
-
-let simp2 #a c f :
-  Lemma((forall (x:a). c == x ==> f x) == f c) = assume False
-
+(* Lots of rewriting rules for the simplifier that we define below *)
 let simplify_pure_null_wp_ax1 #a : Lemma(pure_null_wp a (fun _ -> True) == True) = ()
 
 let simplify_b2t_true () : Lemma(b2t true == True) = ()
+
 let simplify_True_and p : Lemma((True /\ p) == auto_squash p) = ()
+
 let simplify_and_True p : Lemma((p /\ True) == auto_squash p) = ()
+
 let simplify_auto_squash_auto_squash p : Lemma(auto_squash (auto_squash p) == auto_squash p) = ()
 
 let simplify_auto_squash_implies p q : Lemma((auto_squash p ==> q) == (p ==> q)) = ()
+
 let simplify_implies_auto_squash p q : Lemma((p ==> auto_squash q) == (p ==> q)) = ()
 
 let simplfify_eq_true b : Lemma((b = true) == b) = ()
 
-let simplfify_eqq_true b : Lemma((b == true) == b2t b) = admit()
+let simplfify_eqq_true b : Lemma((b == true) == b2t b) by (norm[delta]) = ()
 
 let simplify_lift_pure_prob_wp_auto_squash f : Lemma(lift_pure_prob_wp (fun post -> auto_squash (f post)) == lift_pure_prob_wp (fun post -> f post)) by (admit_all()) = ()
 
-//let simplify_lift_pure_prob_wp_trivial (#a:Type) (x:a) : Lemma(lift_pure_prob_wp (fun (post:pure_post a) -> (post x)) == (fun (post:prob_post a) -> post x)) = admit()
+let simplify_lift_pure_prob_wp_pure_return (#a:Type) (x:a) : Lemma(lift_pure_prob_wp (pure_return a x) == prob_wreturn x) by (admit_all()) = ()
 
-let simplify_lift_pure_prob_wp_pure_return (#a:Type) (x:a) : Lemma(lift_pure_prob_wp (pure_return a x) == prob_wreturn x) by (admit_all()) = admit()
+assume val simplify_pure_return (#a: Type) (x: a) :
+  Lemma((fun post -> post x) == pure_return a x)
 
-let simplify_pure_return (#a: Type) (x: a) :
-  Lemma((fun post -> post x) == pure_return a x) = admit()
+assume val simplify_pure_return' (#a: Type) (x: a) :
+  Lemma((fun post -> auto_squash (post x)) == pure_return a x)
 
-let simplify_pure_return' (#a: Type) (x: a) :
-  Lemma((fun post -> auto_squash (post x)) == pure_return a x) = admit()
-
-let pure_admit_wp (a:Type) : pure_wp a by (admit_all()) = (fun (p: pure_post a) -> True)
-
-let simplify_cond_pure_return (#a: Type) (c: Type) (x: a) :
-  Lemma((fun post -> c ==> post x) == ifte c (pure_return a x) (pure_admit_wp a)) = admit()
-
-//let simplify_pure_return'' () : Lemma((fun post -> auto_squash (post ())) == pure_return unit ()) = simplify_pure_return' ()
-
-let ifte_lift (#a:Type) (#b:Type) (f:a->b) (c:Type) (x y: a) : Lemma(f (ifte c x y) == ifte c (f x) (f y)) = admit()
-
-
-assume val prob_admit_wp : (a:Type) -> prob_wp a (* infinity *)
+assume val simplify_cond_pure_return (#a: Type) (c: Type) (x: a) :
+  Lemma((fun post -> c ==> post x) == ifte c (pure_return a x) (pure_admit_wp a))
+  
+assume val ifte_lift (#a:Type) (#b:Type) (f:a->b) (c:Type) (x y: a) : Lemma(f (ifte c x y) == ifte c (f x) (f y))
 
 let ifte_lift_lift_pure_prob_wp (#a:Type) (c:Type) (x y: pure_wp a) :
   Lemma(lift_pure_prob_wp (ifte c x y) == ifte c (lift_pure_prob_wp x) (lift_pure_prob_wp y)) 
   = ifte_lift lift_pure_prob_wp c x y
 
-
-let ifte_lift_prob_wbind (#a:Type) (#b:Type) (c:Type) (x y: prob_wp a) (wp2:a->prob_wp b):
+assume val ifte_lift_prob_wbind (#a:Type) (#b:Type) (c:Type) (x y: prob_wp a) (wp2:a->prob_wp b):
   Lemma(prob_wbind (ifte c x y) wp2 == ifte c (prob_wbind x wp2) (prob_wbind y wp2)) 
-  = admit()
-
-(*let tmp c = ifte_lift_prob_wbind c
-  (lift_pure_prob_wp (pure_return unit ())) (prob_admit_wp unit)
-                  (fun _ x -> prob_wreturn 0 x)*)
 
 let simplify_if (#a:Type) (c:bool) (t e: bool->a) :
   Lemma((if c then t c else e c) == (if c then t true else e false)) = ()
 
-let lift_pure_prob_wp_pure_admit_wp a : 
-  Lemma(lift_pure_prob_wp (pure_admit_wp a) == prob_admit_wp a) = admit()
+assume val lift_pure_prob_wp_pure_admit_wp (a:Type) : 
+  Lemma(lift_pure_prob_wp (pure_admit_wp a) == prob_admit_wp a)
 
-let prob_wbind_prob_admit (#a:Type) (#b:Type) (wp2:a->prob_wp b) :
-  Lemma(prob_wbind (prob_admit_wp a) wp2 == prob_admit_wp b) = admit()
+assume val prob_wbind_prob_admit (#a:Type) (#b:Type) (wp2:a->prob_wp b) :
+  Lemma(prob_wbind (prob_admit_wp a) wp2 == prob_admit_wp b)
 
-let if_ifte1 (#a:Type) (c:bool) (x y z:a) :
-    Lemma((if c then ifte c x y else z) == (if c then x else z)) = admit()
+assume val if_ifte1 (#a:Type) (c:bool) (x y z:a) :
+    Lemma((if c then ifte c x y else z) == (if c then x else z))
 
-let simp_forall_x_xeqc_fx (#a:Type) (c:a) f :
-    Lemma((forall (x:a). x == c ==> f x) == f c) = admit()
-let simp_forall_x_ceqx_fx (#a:Type) (c:a) f :
-    Lemma((forall (x:a). c == x ==> f x) == f c) = admit()
+assume val simp_forall_x_xeqc_fx (#a:Type) (c:a) (f:a->Type) :
+    Lemma((forall (x:a). x == c ==> f x) == f c)
+    
+assume val simp_forall_x_ceqx_fx (#a:Type) (c:a) (f:a->Type) :
+    Lemma((forall (x:a). c == x ==> f x) == f c)
 
-let simp_forall_k (#a:Type) f g :
+assume val simp_forall_k (#a:Type) (f:a->Type) (g:(a->Type)->Type) :
     Lemma((forall k. (forall (x:a). f x ==> k x) ==> g k) == g f)
-    = admit()
 
-let simp_fun_ite (#a:Type) c f g :
+assume val simp_fun_ite (#a:Type) (c:Type) (f:a->Type) (g:a->Type) :
     Lemma((fun p -> (c ==> f p) /\ (~c ==> g p)) == ifte c f g)
-    = admit()
 
-(*
-/// Runs tac and returns whether tac changed the goal.
-/// Assumes that only the current goal is affected and that the current goal is not removed
-let changed_tac (tac: unit -> Tac unit) : Tac bool =
-    let goal = cur_goal () in
-    tac ();
-    let goal2 = cur_goal () in
-    not (term_eq goal goal2)
-*)
-
-let ifte_inline (#a:Type) c (d:Type->a) (e:Type->a) :
-  Lemma(ifte c (d c) (d c) == ifte c (d True) (d False)) = admit()
-
-// (lift_pure_prob_wp (fun post -> forall (any_result: nat). post any_result))
-
-//let lift_pure_prob_wp #a (wp:pure_wp a) : prob_wp a =
-//    (fun (post:prob_post a) -> largest (fun (p:pr) -> wp (fun x -> p <=. post x)))
+assume val ifte_inline (#a:Type) (c:Type) (d:Type->a) (e:Type->a) :
+  Lemma(ifte c (d c) (d c) == ifte c (d True) (d False))
 
 let lift_pure_prob_wp_inf (#a:Type) :
   Lemma(lift_pure_prob_wp (fun post -> forall (x: a). post x)
      == (fun (post: prob_post a) -> inf post))
-     by (admit_all())
-     = ()
+     by (admit_all()) = ()
 
-assume val ifte_True (a:Type) (x:a) (y:a) : Lemma(ifte True x y == x)
+let ifte_True (a:Type) (x:a) (y:a) : Lemma(ifte True x y == x) = ()
+(* End of simplification rules *)
 
+(* Now I am building a simplifier tactic that applies the rules above.
+   (And does some elementary intro-rules for -> and forall and /\ and (auto_)squash and True as well.)
+   It is quite brute-force and very slow. *)
+
+(* Tries to apply all of the simplification rules once. *)
 let simplifier1 () : Tac unit =
   l_to_r [`simplify_pure_null_wp_ax1];
   l_to_r [`simplify_lift_pure_prob_wp_pure_return];
@@ -348,13 +291,13 @@ let simplifier1 () : Tac unit =
   l_to_r [`ifte_True];
   ()
 
-let forget_result #a #b (tac: a -> Tac b) x : Tac unit = let _ = tac x in ()
-
+// Tactic for removing auto_squash
 let auto_squash_intro_lemma (#a: Type) (x: squash a) : squash (auto_squash a) = ()
-
 let auto_squash_intro () : Tac unit = apply(`auto_squash_intro_lemma)
 
-/// Assumes a focused goal
+// Applies introduction rules to the current goal. This splits a huge goal into independent subgoals.
+// This tactic assumes that there is only one subgoal. 
+// (Can be achieved with the tactics "focus" or "iterAll".)
 let rec intros () : Tac unit =
     match term_as_formula (cur_goal ()) with
       | Implies _ _ -> let _ = implies_intro () in intros ()
@@ -372,12 +315,10 @@ let rec intros () : Tac unit =
             | _ -> ())
       | _ -> ()
 
-
-(*let rec intros () : Tac bool =
-    let one = split <|> forget_result implies_intro <|> forget_result forall_intros <|> double_squash_intro <|> trivial in
-    try one (); iterAll (forget_result intros); true
-    with | _ -> false *)
-
+// Runs the simplifier. Basically, repeatedly runs simplify1 from
+// above, and the builtin simpl() and intros() untol nothing changes
+// any more.
+// This tactic assumes that there is only one subgoal. 
 let rec simplifierFocused () : Tac unit =
   dump "starting simplifier";
   simpl();
@@ -394,28 +335,27 @@ and simplifierFocused' () : Tac unit =
   then ()
   else iterAll simplifierFocused
 
+// Like simplifierFocused, but does not assume a single subgoal (operates on the first)
 let simplifier () : Tac unit =
   focus simplifierFocused
 
+// Like simplifierFocused, but does not assume a single subgoal (operates on all subgoals)
 let simplifierAll () : Tac unit =
   iterAll simplifierFocused
 
+// Helper tactic. Sometimes needed to avoid that SMT does not get
+// invalid terms (see https://github.com/FStarLang/FStar/issues/2299).
+// Can be simply applied at the very end of a tactic.
 let unfold_tac () : Tac unit = norm [delta_qualifier ["unfold"]]
 
+// Testing the simplifier (this does not work without simplifier)
+let test3 x : PROB string (prob_wreturn x) by (simplifier()) = x
 
-// TODO: remove admit_all
-// TODO: move down to the failing things
-let test3 x : PROB string (prob_wreturn x) by (admit_all()) = assume False; x
-
+// Testing if things work
 let test4 () : PROB string (prob_wreturn "hello") = test3 "hello"
 
-
-let test8a c : PROB nat (fun post -> if c then post 0 else post 1)
-   by (simplifier(); cases_bool (quote c); simplifierAll(); dump""; unfold_tac()) =
-  if c then probr 0 else probr 1
-
-
-
+// Testing the simplifier (this does not work without simplifier).
+// We need to manually tell F* to make a case distinction on c. Simplifier is not smart enough.
 let test8b c : PROB nat (fun post -> if c then post 0 else post 1)
    by (cases_bool (quote c);
        simplifierAll();
@@ -423,13 +363,13 @@ let test8b c : PROB nat (fun post -> if c then post 0 else post 1)
   if c then 0 else 1
 
 
-//let strengthen (a b:Type) (p:a -> ProbAny b) (wp:a -> prob_wp b) : (q:(x:a -> PROB b (wp x)){p==q}) = assume False; p
-
-// FAILS
+// Testing the simplifier (this does not work without simplifier).
+// FAILS (when removing admit_all()).
+// Reason: simplifier cannot simplify "ifte c then ...c... else ...c..." 
+//    to "ifte c then ...True... else ...False..."
 let test8 () : PROB nat (fun p -> (p 0 +. p 1) /. two) by (
 simplifier();
-//l_to_r [`ifte_inline];
-smt();
+//smt();
 smt();
 smt();
 dump"";
@@ -438,12 +378,34 @@ admit_all();
 ) =
    let c : bool = coin() in (if c then 0 else 1)
 
-// FAILS
-let test9 () : PROB bool (fun post -> (post true +. post false) /. two) =
+// Testing the simplifier (this does not work without simplifier).
+// FAILS (when removing admit_all()).
+// Haven't investigated the reason yet.
+let test9 () : PROB bool (fun post -> (post true +. post false) /. two)
+by (
+simplifier();
+//smt();
+smt();
+smt();
+dump"";
+admit_all();
+())
+=
   (if coin () then coin() else coin())
 
-// FAILS
-let test10 () : PROB nat (fun p -> (p 0 +. p 1) /. two) =
+// Testing the simplifier (this does not work without simplifier).
+// FAILS (when removing admit_all()).
+// Haven't investigated the reason yet.
+let test10 () : PROB nat (fun p -> (p 0 +. p 1) /. two) 
+by (
+simplifier();
+//smt();
+smt();
+smt();
+dump"";
+admit_all();
+())
+=
   let c : bool = coin() in
   (if true then 0 else 1)
 
